Lemke/FiniteAutomaton.thy
@@ -1,10 +1,25 @@
 section\<open>Finite Automata\<close>
 
+text\<open>
+  The fact that for a regular language \<open>L\<close>, the predecessors with respect to a context-free grammar
+  \<open>pre\<^sup>*(L)\<close> is also regular has been discovered independently by many authors \cite{book1993string, buchi3105regular, caucal1992regular}.
+  This represents a key closure property, since the word-problem for regular languages is
+  inherently decidable, as are many other problems.
+  To reason about regular languages, a simple model of a non-deterministic finite automaton (NFA)
+  without \<open>\<epsilon>\<close>-transitions is defined.
+\<close>
+
 theory FiniteAutomaton
   imports Main
 begin \<comment>\<open>begin-theory FiniteAutomaton\<close>
 
 subsection\<open>Definition\<close>
+
+text\<open>
+  In this theory, an NFA \<open>M\<close> is defined as the \<open>3\<close>-tuple \<open>(\<delta>, S, F)\<close>, where \<open>\<delta>\<close> are the transitions,
+  \<open>S\<close> is the starting symbol and \<open>F\<close> are the final states. The state-domain \<open>Q\<close> and alphabet \<open>\<Sigma>\<close>
+  are not explicitly given, since the type-theory still allows for proof of formal correctness.
+\<close>
 
 record ('s, 't) nfa =
   transitions :: "('s \<times> 't \<times> 's) set"
@@ -13,33 +28,52 @@ record ('s, 't) nfa =
 
 subsection\<open>Step Relation\<close>
 
-definition step :: "('s \<times> 't \<times> 's) set \<Rightarrow> 't \<Rightarrow> 's \<Rightarrow> 's set" where
-  "step T c s = { s'. (s, c, s') \<in> T }"
+text\<open>
+  The following two lemmas ensure that Isabelle can automatically evaluate set expressions with
+  \<open>2\<close>-tuples and \<open>3\<close>-tuples, which will be used thouroughly within this project.
+\<close>
 
-lemma step_code[code]: "step T c s = (snd o snd) ` {t \<in> T. case t of (st,ct,st') \<Rightarrow> st = s \<and> ct = c}"
-  unfolding step_def by (auto simp: image_iff split: prod.splits)
+lemma [code_unfold]:
+  "{(x,y) \<in> A. P x y} = {p \<in> A. P (fst p) (snd p)}"
+  by fastforce
+
+lemma [code_unfold]:
+  "{(x,y,z) \<in> A. P x y z} = {p \<in> A. P (fst p) (fst (snd p)) (snd (snd p))}"
+  by fastforce
+
+text\<open>
+  A step from a single state \<open>q\<close> over a single symbol \<open>c\<close> is the set of all \<open>q'\<close>, where \<open>(q, c, q') \<in> \<delta>\<close>:
+\<close>
+
+definition step :: "('s \<times> 't \<times> 's) set \<Rightarrow> 't \<Rightarrow> 's \<Rightarrow> 's set" where
+  "step T c s = (\<lambda>(q, c, q'). q') ` {(q, c', q') \<in> T. c = c' \<and> q = s}"
+
+text\<open>
+  A step of a single symbol \<open>c\<close> from a set of states \<open>S\<close> is the union of @{term step} over \<open>S\<close>:
+\<close>
 
 definition Step :: "('s \<times> 't \<times> 's) set \<Rightarrow> 't \<Rightarrow> 's set \<Rightarrow> 's set" where
-  "Step T c s = { s'. \<exists>s\<^sub>0 \<in> s. s' \<in> step T c s\<^sub>0 }"
+  "Step T c S = \<Union>((\<lambda>s. step T c s) ` S)"
 
-lemma Step_code[code]: "Step T c s = (\<Union>s\<^sub>0 \<in> s. step T c s\<^sub>0)"
-  unfolding Step_def by (auto)
+text\<open>
+  Repeated steps of a word \<open>w\<close> consisting of multiple letters is achieved using a standard @{term fold}:
+\<close>
 
 definition Steps :: "('s \<times> 't \<times> 's) set \<Rightarrow> 't list \<Rightarrow> 's set \<Rightarrow> 's set" where
   "Steps T w s = fold (Step T) w s"
 
+text\<open>
+  However, we often only regard a single-starting state, for which the following abbreviation is introduced:
+\<close>
+
 abbreviation steps :: "('s \<times> 't \<times> 's) set \<Rightarrow> 't list \<Rightarrow> 's \<Rightarrow> 's set" where
   "steps T w s \<equiv> Steps T w {s}"
-
-value "steps {(0,CHR ''a'',0)} ([CHR ''a'',CHR ''a'']::char list) (0::int)"
 
 lemma Step_union: "Step T w (S\<^sub>1 \<union> S\<^sub>2) = Step T w S\<^sub>1 \<union> Step T w S\<^sub>2"
   unfolding Step_def by blast
 
-lemma Steps_mono:
-  assumes "s\<^sub>1 \<subseteq> s\<^sub>2"
-  shows "Steps T w s\<^sub>1 \<subseteq> Steps T w s\<^sub>2"
-proof (insert assms; induction w arbitrary: s\<^sub>1 s\<^sub>2)
+lemma Steps_mono: "s\<^sub>1 \<subseteq> s\<^sub>2 \<Longrightarrow> Steps T w s\<^sub>1 \<subseteq> Steps T w s\<^sub>2"
+proof (induction w arbitrary: s\<^sub>1 s\<^sub>2)
   case Nil thus ?case by (simp add: Steps_def)
 next
   case (Cons w ws)
@@ -59,8 +93,7 @@ next
     by simp
 qed
 
-\<comment>\<open>Sanity check that a monotonicity rule is really defined:\<close>
-lemma [mono]: "mono (Steps T w)"
+lemma [mono]: "mono (Steps T w)" (* TODO: give proper name to lemma *)
   by (intro monoI, elim Steps_mono)
 
 lemma Steps_path:
@@ -124,25 +157,31 @@ qed
 lemma Steps_split3:
   assumes "q\<^sub>f \<in> Steps T (w\<^sub>1@w\<^sub>2@w\<^sub>3) Q\<^sub>0"
   shows "\<exists>q' q''. q' \<in> Steps T w\<^sub>1 Q\<^sub>0 \<and> q'' \<in> steps T w\<^sub>2 q' \<and> q\<^sub>f \<in> steps T w\<^sub>3 q''"
-  using assms Steps_split by meson
+proof -
+  obtain q' where "q' \<in> Steps T (w\<^sub>1@w\<^sub>2) Q\<^sub>0 \<and> q\<^sub>f \<in> steps T w\<^sub>3 q'"
+    using assms Steps_split[where w\<^sub>1 = "w\<^sub>1@w\<^sub>2"] by fastforce
+  moreover obtain q'' where "q'' \<in> Steps T w\<^sub>1 Q\<^sub>0 \<and> q' \<in> steps T w\<^sub>2 q''"
+    using calculation Steps_split by fast
+  ultimately show ?thesis
+    by blast
+qed
 
 lemma Steps_join3:
   assumes "q' \<in> steps T w\<^sub>1 q\<^sub>0" and "q'' \<in> steps T w\<^sub>2 q'" and "q\<^sub>f \<in> steps T w\<^sub>3 q''"
   shows "q\<^sub>f \<in> steps T (w\<^sub>1@w\<^sub>2@w\<^sub>3) q\<^sub>0"
-  using assms Steps_join by metis
+proof -
+  have "q\<^sub>f \<in> steps T (w\<^sub>2@w\<^sub>3) q'"
+    using assms(2) assms(3) Steps_join by fast
+  moreover have "q\<^sub>f \<in> steps T (w\<^sub>1@w\<^sub>2@w\<^sub>3) q\<^sub>0"
+    using calculation assms(1) Steps_join by fast
+  ultimately show ?thesis
+    by blast
+qed
 
 subsection\<open>Language\<close>
 
 abbreviation accepts :: "('s \<times> 't \<times> 's) set \<Rightarrow> 's \<Rightarrow> 's set \<Rightarrow> 't list \<Rightarrow> bool" where
   "accepts T s F w \<equiv> (steps T w s \<inter> F \<noteq> {})"
-
-(* Two example evaluations/tests *)
-
-lemma "accepts {(0::int,CHR ''a'',0), (0::int,CHR ''a'',1)} 0 {0} [CHR ''a'',CHR ''a'']"
-  by eval
-
-lemma "\<not> accepts {(0::int,CHR ''a'',0), (0::int,CHR ''b'',1)} 0 {0} [CHR ''b'',CHR ''a'']"
-  by eval
 
 lemma accepts_split3:
   assumes "accepts T s F (w\<^sub>1@w\<^sub>2@w\<^sub>3)"
@@ -179,6 +218,140 @@ proof -
     unfolding lang'_def using \<open>q\<^sub>f \<in> F\<close> calculation by blast
   ultimately show ?thesis
     using that by blast
+qed
+
+lemma nfa_mono':
+  assumes "T\<^sub>1 \<subseteq> T\<^sub>2" and "q\<^sub>1 \<subseteq> q\<^sub>2"
+  shows "Steps T\<^sub>1 w q\<^sub>1 \<subseteq> Steps T\<^sub>2 w q\<^sub>2"
+proof (insert assms(2); induction w arbitrary: q\<^sub>1 q\<^sub>2)
+  case Nil thus ?case by (simp add: Steps_def)
+next
+  case (Cons w ws)
+  have "Step T\<^sub>1 w q\<^sub>1 \<subseteq> Step T\<^sub>2 w q\<^sub>2"
+    unfolding Step_def step_def using assms(1) Cons(2) by blast
+  then have "Steps T\<^sub>1 ws (Step T\<^sub>1 w q\<^sub>1) \<subseteq> Steps T\<^sub>1 ws (Step T\<^sub>2 w q\<^sub>2)"
+    by (rule Steps_mono)
+  then have "Steps T\<^sub>1 ws (Step T\<^sub>1 w q\<^sub>1) \<subseteq> Steps T\<^sub>2 ws (Step T\<^sub>2 w q\<^sub>2)"
+    using Cons(1) by blast
+  then show ?case
+    by (simp add: Steps_def)
+qed
+
+lemma nfa_mono: "T\<^sub>1 \<subseteq> T\<^sub>2 \<Longrightarrow> steps T\<^sub>1 w q \<subseteq> steps T\<^sub>2 w q"
+  using nfa_mono'[of T\<^sub>1 T\<^sub>2 "{q}" "{q}" w] by simp
+
+lemma nfa_steps_mono: "\<delta>\<^sub>1 \<subseteq> \<delta>\<^sub>2 \<Longrightarrow> q' \<in> steps \<delta>\<^sub>1 w q \<Longrightarrow> q' \<in> steps \<delta>\<^sub>2 w q"
+proof -
+  assume "\<delta>\<^sub>1 \<subseteq> \<delta>\<^sub>2"
+  then have "steps \<delta>\<^sub>1 w q \<subseteq> steps \<delta>\<^sub>2 w q"
+    by (rule nfa_mono)
+  then show "q' \<in> steps \<delta>\<^sub>1 w q \<Longrightarrow> q' \<in> steps \<delta>\<^sub>2 w q"
+    by blast
+qed
+
+lemma nfa_steps_union: "q' \<in> steps \<delta> w q \<Longrightarrow> q' \<in> steps (\<delta> \<union> \<delta>') w q"
+proof -
+  have "\<delta> \<subseteq> (\<delta> \<union> \<delta>')"
+    by simp
+  then show "q' \<in> steps \<delta> w q \<Longrightarrow> q' \<in> steps (\<delta> \<union> \<delta>') w q"
+    by (rule nfa_steps_mono)
+qed
+
+lemma nfa_lang_mono: "T\<^sub>1 \<subseteq> T\<^sub>2 \<Longrightarrow> lang' T\<^sub>1 s f \<subseteq> lang' T\<^sub>2 s f"
+  unfolding lang'_def using nfa_mono[of T\<^sub>1 T\<^sub>2] by fast
+
+subsection\<open>Reachable States\<close>
+
+type_synonym ('s, 't) Trans = "('s \<times> 't \<times> 's) set"
+
+definition reachable_from :: "('s, 't) Trans \<Rightarrow> 's \<Rightarrow> 's set" where
+  "reachable_from \<delta> q \<equiv> {q'. \<exists>w. q' \<in> steps \<delta> w q}"
+
+lemma reachable_from_computable: "reachable_from \<delta> q \<subseteq> {q} \<union> (snd ` snd ` \<delta>)"
+proof
+  fix q'
+  assume "q' \<in> reachable_from \<delta> q"
+  then obtain w where w_def: "q' \<in> steps \<delta> w q"
+    unfolding reachable_from_def by blast
+  then consider "w = []" | "\<exists>ws c. w = ws@[c]"
+    by (meson rev_exhaust)
+  then show "q' \<in> {q} \<union> (snd ` snd ` \<delta>)"
+  proof (cases)
+    case 1
+    then show ?thesis
+      using w_def Steps_def by force
+  next
+    case 2
+    then obtain ws c where "w = ws@[c]"
+      by blast
+    then obtain q1 where "q1 \<in> steps \<delta> ws q" and "q' \<in> steps \<delta> [c] q1"
+      using Steps_split w_def by fast
+    then have "(q1, c, q') \<in> \<delta>"
+      by (auto simp: Steps_def Step_def step_def)
+    then show ?thesis
+      by force
+  qed
+qed
+
+lemma reachable_from_trans[trans]:
+  assumes "q1 \<in> reachable_from \<delta> q0" and "q2 \<in> reachable_from \<delta> q1"
+  shows "q2 \<in> reachable_from \<delta> q0"
+  using assms Steps_join unfolding reachable_from_def by fast
+
+lemma reachable_add_trans:
+  assumes "\<forall>(q1, _, q2) \<in> \<delta>'. \<exists>w. q2 \<in> steps \<delta> w q1"
+  shows "reachable_from \<delta> q = reachable_from (\<delta> \<union> \<delta>') q"
+proof (standard; standard)
+  fix q'
+  assume "q' \<in> reachable_from \<delta> q"
+  then show "q' \<in> reachable_from (\<delta> \<union> \<delta>') q"
+    unfolding reachable_from_def using nfa_steps_union by fast
+next
+  fix q'
+  assume "q' \<in> reachable_from (\<delta> \<union> \<delta>') q"
+  then obtain w where "q' \<in> steps (\<delta> \<union> \<delta>') w q"
+    unfolding reachable_from_def by blast
+  then have "\<exists>w'. q' \<in> steps \<delta> w' q"
+  proof (induction w arbitrary: q)
+    case Nil
+    then have "q = q'" and "q \<in> steps \<delta> [] q"
+      unfolding Steps_def by simp+
+    then show ?case
+      by blast
+  next
+    case (Cons c w)
+    then obtain q1 where "q' \<in> steps (\<delta> \<union> \<delta>') w q1" and "q1 \<in> steps (\<delta> \<union> \<delta>') [c] q"
+      using Steps_split[where w\<^sub>1="[c]" and w\<^sub>2=w] by force
+    then obtain w' where w'_def: "q' \<in> steps \<delta> w' q1"
+      using Cons by blast
+
+    have "q1 \<in> step (\<delta> \<union> \<delta>') c q"
+      using \<open>q1 \<in> steps (\<delta> \<union> \<delta>') [c] q\<close> by (simp add: Steps_def Step_def)
+    then consider "q1 \<in> step \<delta> c q" | "q1 \<in> step \<delta>' c q"
+      unfolding step_def by blast
+    then show ?case
+    proof (cases)
+      case 1
+      then have "q1 \<in> steps \<delta> [c] q"
+        by (simp add: Steps_def Step_def)
+      then have "q' \<in> steps \<delta> (c#w') q"
+        using w'_def Steps_join by force
+      then show ?thesis
+        by blast
+    next
+      case 2
+      then have "(q, c, q1) \<in> \<delta>'"
+        by (auto simp: step_def)
+      then obtain w'' where "q1 \<in> steps \<delta> w'' q"
+        using assms by blast
+      then have "q' \<in> steps \<delta> (w''@w') q"
+        using w'_def Steps_join by fast
+      then show ?thesis
+        by blast
+    qed
+  qed
+  then show "q' \<in> reachable_from \<delta> q"
+    by (simp add: reachable_from_def)
 qed
 
 end \<comment>\<open>end-theory FiniteAutomaton\<close>
