Lemke/Applications.thy
@@ -1,17 +1,23 @@
 section\<open>Applications\<close>
+text\<open>\label{sec:applications}\<close>
 
 theory Applications
-  imports Definition Finiteness
+  imports Definition
 begin \<comment>\<open>begin-theory Applications\<close>
 
 subsection\<open>Membership Problem\<close>
 
-theorem (in CFG) "w \<in> Lang P S \<longleftrightarrow> [(Nt S)] \<in> pre_star {map_word w}"
-  unfolding Lang_def pre_star_def by (simp add: derives_eq)
+locale CFG =
+  fixes P :: "('n, 't) Prods"
+    and S :: 'n
+begin
+
+theorem "w \<in> Lang P S \<longleftrightarrow> [(Nt S)] \<in> pre_star P {map_word w}"
+  unfolding Lang_def pre_star_def by simp
 
 subsection\<open>Subset Problem\<close>
 
-theorem (in CFG) "Lang P S \<subseteq> L \<longleftrightarrow> [(Nt S)] \<notin> pre_star (map_lang (-L))"
+theorem "Lang P S \<subseteq> L \<longleftrightarrow> [(Nt S)] \<notin> pre_star P (map_lang (-L))"
 proof -
   have "Lang P S \<subseteq> L \<longleftrightarrow> Lang P S \<inter> -L = {}"
     by blast
@@ -21,40 +27,40 @@ qed
 
 subsection\<open>Disjointness Problem\<close>
 
-theorem (in CFG) "Lang P S \<inter> L = {} \<longleftrightarrow> [(Nt S)] \<notin> pre_star (map_lang L)"
+theorem "Lang P S \<inter> L = {} \<longleftrightarrow> [(Nt S)] \<notin> pre_star P (map_lang L)"
   by (simp add: pre_star_lang)
 
 subsection\<open>Emptiness Problem\<close>
 
-theorem (in CFG) "Lang P S = {} \<longleftrightarrow> [(Nt S)] \<notin> pre_star (map_lang UNIV)"
+theorem "Lang P S = {} \<longleftrightarrow> [(Nt S)] \<notin> pre_star P (map_lang UNIV)"
 proof -
   have "Lang P S = {} \<longleftrightarrow> Lang P S \<subseteq> {}"
     by blast
   then have "Lang P S = {} \<longleftrightarrow> Lang P S \<inter> UNIV = {}"
     by blast
   then show ?thesis
-    using pre_star_lang[of UNIV] by simp
+    using pre_star_lang[of P S UNIV] by simp
 qed
 
 subsection\<open>Useless Variables\<close>
 
-theorem (in CFG) "is_reachable X \<longleftrightarrow> [Nt S] \<in> pre_star { \<alpha>@[Nt X]@\<beta> | \<alpha> \<beta>. True }"
+theorem "(P \<turnstile> S \<Rightarrow>\<^sup>? X) \<longleftrightarrow> [Nt S] \<in> pre_star P { \<alpha>@[Nt X]@\<beta> | \<alpha> \<beta>. True }"
 proof -
   define L where "L \<equiv> { (\<alpha>::('n, 't) syms)@[Nt X]@\<beta> | \<alpha> \<beta>. True }"
-  have "[Nt S] \<in> pre_star L  \<longleftrightarrow> (\<exists>w. w \<in> L \<and> [Nt S] \<Rightarrow>\<^sup>* w)"
+  have "[Nt S] \<in> pre_star P L  \<longleftrightarrow> (\<exists>w. w \<in> L \<and> P \<turnstile> [Nt S] \<Rightarrow>* w)"
     by (simp add: pre_star_term)
-  also have "... \<longleftrightarrow> (\<exists>\<alpha> \<beta>. [Nt S] \<Rightarrow>\<^sup>* (\<alpha>@[Nt X]@\<beta>))"
+  also have "... \<longleftrightarrow> (\<exists>\<alpha> \<beta>. P \<turnstile> [Nt S] \<Rightarrow>* (\<alpha>@[Nt X]@\<beta>))"
     unfolding L_def by blast
   finally show ?thesis
-    by (simp add: is_reachable_def is_reachable_from_def L_def)
+    by (simp add: is_reachable_from_def L_def)
 qed
 
-theorem (in CFG) "is_productive X \<longleftrightarrow> [Nt X] \<in> pre_star { map_word w | w. True }"
+theorem "is_productive P X \<longleftrightarrow> [Nt X] \<in> pre_star P { map_word w | w. True }"
 proof -
-  define L where "L \<equiv> { map_word w | w. True }"
-  have "[Nt X] \<in> pre_star L \<longleftrightarrow> (\<exists>w. w \<in> L \<and> [Nt X] \<Rightarrow>\<^sup>* w)"
+  define L :: "('n, 't) sym list set" where "L \<equiv> { map_word w | w. True }"
+  have "[Nt X] \<in> pre_star P L \<longleftrightarrow> (\<exists>w. w \<in> L \<and> P \<turnstile> [Nt X] \<Rightarrow>* w)"
     by (simp add: pre_star_term)
-  also have "... \<longleftrightarrow> (\<exists>w. [Nt X] \<Rightarrow>\<^sup>* map_word w)"
+  also have "... \<longleftrightarrow> (\<exists>w. P \<turnstile> [Nt X] \<Rightarrow>* map_word w)"
     unfolding L_def by blast
   finally show ?thesis
     by (simp add: is_productive_def L_def)
@@ -62,23 +68,14 @@ qed
 
 subsection\<open>Nullable Variables\<close>
 
-theorem (in CFG) "is_nullable X \<longleftrightarrow> [Nt X] \<in> pre_star {[]}"
+theorem "is_nullable P X \<longleftrightarrow> [Nt X] \<in> pre_star P {[]}"
 proof -
-  have "[Nt X] \<in> pre_star {[]} \<longleftrightarrow> (\<exists>w. w \<in> {[]} \<and> [Nt X] \<Rightarrow>\<^sup>* w)"
+  have "[Nt X] \<in> pre_star P {[]} \<longleftrightarrow> (\<exists>w. w \<in> {[]} \<and> P \<turnstile> [Nt X] \<Rightarrow>* w)"
     by (simp add: pre_star_term)
   then show ?thesis
     by (simp add: is_nullable_def)
 qed
 
-subsection\<open>Finiteness Problem\<close>
-
-lemma (in CFG) is_infinite_check:
-  "is_infinite \<longleftrightarrow> (\<exists>X. [Nt X] \<in> pre_star { \<alpha>@[Nt X]@\<beta> | \<alpha> \<beta>. \<alpha>@\<beta> \<noteq> [] })"
-  unfolding is_infinite_def is_reachable_step_def by (auto simp: pre_star_term)
-
-theorem (in CFG) is_infinite_by_prestar:
-  assumes "is_useful_all" and "is_non_nullable_all"
-  shows "finite (Lang P S) \<longleftrightarrow> (\<forall>X. [Nt X] \<notin> pre_star { \<alpha>@[Nt X]@\<beta> | \<alpha> \<beta>. \<alpha>@\<beta> \<noteq> [] })"
-  using assms is_infinite is_infinite_check by blast
+end
 
 end \<comment>\<open>end-theory Applications\<close>
